Plausible liveness, with a few unproved lemmas.

Core/PlausibleLiveness.v
@@ -4,6 +4,9 @@ Require Import all_ssreflect.
 From Hammer
 Require Import Hammer Reconstr.
 
+From mathcomp
+     Require Import finmap.
+
 Set Implicit Arguments.
 Unset Strict Implicit.
 Unset Printing Implicit Defensive.
@@ -13,19 +16,80 @@ Section Liveness.
 Variable Validator : finType.
 Variable Hash : finType.
 
+(* "2/3", quorums sufficient to "justify" a link *)
 Variable quorum_1 : {set {set Validator}}.
+(* "1/3" we will assume each of these sets contains at least one good node *)
 Variable quorum_2 : {set {set Validator}}.
 
-(* vote_msg node hash view view_src *)
-Record State :=
- { vote_msg : Validator -> Hash -> nat -> nat -> bool }.
+(* The essential property behind 2/3+1/3 - any two sets from quoroum_1
+   have as common members the entire contents of some quorum_2 set,
+   so any two decisions each with quorum_1-set have overlapping support
+   of at least some quorum_2-set, and then of one good node *)
+Hypothesis quorums_intersection :
+  forall q1 q2, q1 \in quorum_1 -> q2 \in quorum_1 ->
+  exists q3, q3 \in quorum_2 /\ q3 \subset q1 /\ q3 \subset q2.
 
+Hypothesis quorum_2_nonempty:
+  forall q, q \in quorum_2 -> exists v, v \in q.
+
+Hypothesis quorum_1_nonempty:
+  forall q, q \in quorum_1 -> exists v, v \in q.
+
+(*
+Lemma quorum_1_nonempty:
+  forall q, q \in quorum_1 -> exists v, v \in q.
+Proof.
+  intros.
+  destruct (quorums_intersection H H) as (q2 & Hq2 & Hsub & _).
+  clear H.
+  apply quorum_2_nonempty in Hq2.
+  destruct Hq2. exists x.
+  revert H.
+  apply (subsetP Hsub).
+Qed.
+ *)
+
+(*
+Lemma quorums_property :
+ forall q1 q2, q1 \in quorum_1 -> q2 \in quorum_1 ->
+ exists q3, q3 \in quorum_2 /\ forall n, n \in q3 -> n \in q1 /\ n \in q2.
+Proof.
+move => q1 q2 Hq1 Hq2.
+have [q3 [Hq3 [Hq13 Hq23]]] := (quorums_intersection Hq1 Hq2).
+exists q3.
+split => //.
+move => n Hn.
+split.
+- by apply/(subsetP Hq13).
+- by apply/(subsetP Hq23).
+Qed.
+*)
+
+(* Each vote names source and target nodes by giving hash and height,
+   and is signed by a particular validator *)
+Definition Vote := (Validator * Hash * Hash * nat * nat)%type.
+(* A state includes a finite set of Votes cast in the current epoch *)
+Definition State := {fset Vote}.
+
+Definition vote_target_height (v:Vote) : nat :=
+  match v with
+    (_,_,_,_,t_h) => t_h
+  end.
+
+Definition vote_msg (st:State) v s t (s_h t_h:nat) : bool
+  := (v,s,t,s_h,t_h) \in st.
+
+(* This relation links blocks (b,b') if b is an ancestor of b' and
+   b' is at the next checkpoint level above b *)
 Variable hash_parent : rel Hash.
 
 Notation "h1 <~ h2" := (hash_parent h1 h2) (at level 50).
 
+(* The genesis block. Usually less interesting than
+   the block which started the current epoch *)
 Variable genesis : Hash.
 
+(* This looks like a very weak fragment of acylic? *)
 Hypothesis hash_at_most_one_parent_1 :
   forall h1 h2, h1 <~ h2 -> h1 <> h2.
 
@@ -71,9 +135,8 @@ Qed.
 Lemma hash_ancestor_other:
   forall h1 h2 p, h1 <~* h2 -> p </~* h2 -> p </~* h1.
 Proof.
-move => h1 h2 p H1 H2.
-move => Hp.
-case: H2.
+move => h1 h2 p H1 H2 Hp.
+destruct H2.
 move: Hp H1.
 by apply/connect_trans.
 Qed.
@@ -85,43 +148,313 @@ Inductive nth_ancestor : nat -> Hash -> Hash -> Prop :=
     nth_ancestor n h1 h2 -> h2 <~ h3 ->
     nth_ancestor n.+1 h1 h3.
 
-Definition slashed_dbl_vote s n :=
- exists h1 h2, h1 <> h2 /\ exists v s1 s2, vote_msg s n h1 v s1 /\ vote_msg s n h2 v s2.
+Hypothesis hash_at_most_one_level:
+  forall h n1 n2,
+    nth_ancestor n1 genesis h ->
+    nth_ancestor n2 genesis h ->
+    n1 = n2.
 
-Definition slashed_surround s n :=
-  exists h1 h2 v1 v2 s1 s2,
-    vote_msg s n h1 v1 s1 /\
-     vote_msg s n h2 v2 s2 /\
-     v1 > v2 /\ s2 > s1.
+(* A validator may not make two votes with different target hashes at the same
+  target height (whatever the source blocks)
+ *)
+Definition slashed_dbl_vote st v :=
+  exists t1 t2, t1 <> t2 /\ exists s1 s1_h s2 s2_h t_h,
+      vote_msg st v s1 t1 s1_h t_h /\ vote_msg st v s2 t2 s2_h t_h.
 
-Definition slashed s n : Prop :=
- slashed_dbl_vote s n \/ slashed_surround s n.
+(* A validator may not make two votes with the source and target of one vote
+   both strictly between the source and target of the other
+ *)
+Definition slashed_surround st v :=
+  exists s1 t1 s1_h t1_h,
+  exists s2 t2 s2_h t2_h,
+    vote_msg st v s1 t1 s1_h t1_h /\
+     vote_msg st v s2 t2 s2_h t2_h /\
+     s2_h > s1_h /\ t2_h < t1_h.
 
-Definition one_third_slashed s :=
- exists q, q \in quorum_2 /\ forall n, n \in q -> slashed s n.
+Definition slashed st v : Prop :=
+ slashed_dbl_vote st v \/ slashed_surround st v.
 
-Definition unslashed_can_extend (s s' : State) := True.
+(* The finalized node at which the current epoch started *)
+Variable epoch_start : Hash.
+Variable epoch_height : nat.
+Hypothesis epoch_ancestry : nth_ancestor epoch_height genesis epoch_start.
 
-Definition no_new_slashed (s s' : State) := True.
-  
-Lemma plausible_liveness :
-  forall s, ~ one_third_slashed s ->
-  exists s', unslashed_can_extend s s' /\
-  no_new_slashed s s'.
+Definition link_supporters st s t s_h t_h : {set Validator} :=
+  [set v | vote_msg st v s t s_h t_h ].
+Definition justified_link (st:State) (s t : Hash) (s_h t_h : nat) : bool :=
+  link_supporters st s t s_h t_h \in quorum_1.
+
+Inductive justified_this_epoch (st:State) : Hash -> nat -> Prop :=
+| epoch_justified : justified_this_epoch st epoch_start epoch_height
+| justfied_link : forall s s_h t t_h,
+    justified_this_epoch st s s_h ->
+    s <~* t ->
+    justified_link st s t s_h t_h ->
+    justified_this_epoch st t t_h.
+
+Lemma justified_is_descendant st n n_h:
+  justified_this_epoch st n n_h -> epoch_start <~* n.
 Proof.
+  induction 1;[
+    eapply connect0|
+    eapply connect_trans; eassumption].
+Defined.
+
+Definition sources_justified st v :=
+  forall s t s_h t_h,
+    vote_msg st v s t s_h t_h ->
+    epoch_start <~* s /\ justified_this_epoch st s s_h.
+
+Definition one_third_slahsed st :=
+  exists q, q \in quorum_2 /\ forall v, v \in q -> slashed st v.
+
+Definition one_third_bad st :=
+  exists q, q \in quorum_2 /\ forall v, v \in q ->
+   (slashed st v \/ ~sources_justified st v).
+
+Definition unslashed_can_extend st st' : Prop :=
+  forall v s t s_h t_h,
+    vote_msg st' v s t s_h t_h = true ->
+    vote_msg st v s t s_h t_h = true \/ ~slashed st v.
+
+Definition no_new_slashed st st' :=
+  forall v, slashed st' v -> slashed st v.
+
+Definition blocks_exist_high_over (base : Hash) : Prop :=
+  forall n, exists block, nth_ancestor n base block.
+
+Definition highest_justified st b b_h : Prop :=
+  forall b' b_h', b_h' >= b_h -> justified_this_epoch st b' b_h' ->
+                  b' == b /\ b_h' == b_h.
+
+Lemma highest_exists: forall st,
+    ~one_third_bad st ->
+    exists b b_h,
+      justified_this_epoch st b b_h /\
+      highest_justified st b b_h.
 Admitted.
 
-(*
-lemma plausible_liveness :
-  "situation_has_finitely_many_validators s \<Longrightarrow>
-   no_invalid_view s \<Longrightarrow>
-   new_descendant_available s \<Longrightarrow>
-   finite_messages s \<Longrightarrow>
-   \<not> one_third_slashed s \<Longrightarrow>
-   \<exists> s_new h_new.
-     \<not> committed s h_new \<and>
-     unslashed_can_extend s s_new \<and>
-     committed s_new h_new \<and>
-     no_new_slashed s s_new"
-*)
+Definition highest (A : {fset nat}) : nat :=
+  \max_(i : [finType of A]) (val i).
+
+Lemma max_nat : forall (s : {fset nat}) (n : nat),
+ n \in s ->
+ n <= \max_(i : s) (val i).
+Proof.
+intro s.
+move => n Hn.
+case (insubP [subType of s] n) => /=; last by move: Hn =>->.
+move => k Hk =><-.
+exact: leq_bigmax_cond.
+Qed.
+
+
+Lemma highest_ub:
+  forall (A : {fset nat}) (x:nat),
+    x \in A -> x <= highest A.
+Proof.
+  apply max_nat.
+Qed.
+
+Lemma two_thirds_good: forall st,
+    ~one_third_bad st ->
+    exists (q : {set Validator}), q \in quorum_1 /\ forall v, v \in q ->
+     (~slashed st v /\ sources_justified st v).
+Admitted.
+
+Lemma ltSnn: forall n, (n.+1 < n) = false.
+Proof.
+  intro n.
+  generalize (ltnn n).
+  apply contraFF.
+  intro.
+  apply ltn_trans with n.+1. apply ltnSn. assumption.
+Qed.
+
+Lemma plausible_liveness :
+  forall st, ~ one_third_bad st ->
+  (forall b b_h, highest_justified st b b_h -> blocks_exist_high_over b) ->
+  exists st', unslashed_can_extend st st' /\ no_new_slashed st st'.
+Proof.
+  intros st Hgood Hheight.
+  destruct (highest_exists Hgood) as (just_max & just_max_h & [Hjust_max_just Hjust_max_max]).
+  specialize (Hheight _ _ Hjust_max_max).
+
+  apply two_thirds_good in Hgood.
+  destruct Hgood as (good_quorum & Hgood_is_quorum & Hgood).
+
+  pose targets := (epoch_height |` [ fset vote_target_height vote | vote in st])%fset;
+                    change {fset nat} in (type of targets).
+  pose highest_target := highest targets.
+  destruct (Hheight (highest_target.+2)) as [new_finalized Hpath].
+  inversion Hpath;subst. rename h2 into new_final_parent.
+
+  pose new_votes1 := [fset (v,just_max,new_final_parent,just_max_h,highest_target.+1)
+                     | v in good_quorum]%fset; change {fset Vote} in (type of new_votes1).
+  pose new_votes2 := [fset (v,new_final_parent,new_finalized,highest_target.+1,highest_target.+2)
+                     | v in good_quorum]%fset; change {fset Vote} in (type of new_votes2).
+
+  exists (st `|` new_votes1 `|` new_votes2)%fset.
+  split.
+  unfold unslashed_can_extend.
+
+  clear -Hgood.
+  unfold vote_msg.
+  intros v s t s_h t_h.
+  rewrite in_fsetU. rewrite in_fsetU.
+  rewrite !Bool.orb_true_iff.
+  move => [[H|H] | H];[tauto|right;apply Hgood..].
+  case/imfsetP: H => x Hx Heq. replace v with x. assumption. congruence.
+  case/imfsetP: H => x Hx Heq. replace v with x. assumption. congruence.
+
+  pose proof (@highest_ub targets).
+  assert (forall v s t s_h t_h, (v,s,t,s_h,t_h) \in st -> t_h <= highest_target)
+    as H_st_highest by
+   (clear;intros;apply highest_ub;
+    apply/fsetUP;right;revert H;apply in_imfset).
+
+  Local Ltac new_vote_mem_tac Hvote :=
+    let x := fresh "x" in
+    let x_good := fresh "x_good" in
+    let Heq := fresh "Heq" in
+    case/imfsetP: Hvote => x x_good Heq;injection Heq;clear Heq;intros;subst x;subst.
+  assert (forall n n_h, justified_this_epoch st n n_h -> n_h <= highest_target)
+    as Hjust_le_target by
+     (clear -quorum_1_nonempty;intros n n_h H;
+     apply highest_ub;destruct H;[by apply fset1U1|];
+     destruct (quorum_1_nonempty H1) as [t_supporter Ht];
+     rewrite in_set in Ht; apply/fsetUP; right;
+     revert Ht; apply in_imfset).
+
+  unfold no_new_slashed.
+  intros badV [Hdbl|Hnest];[left|right].
+  (* slashed for double vote *)
+  unfold slashed_dbl_vote, vote_msg in Hdbl |- *.
+  destruct Hdbl as (t1 & t2 & Hneq_t & Hdouble_votes).
+  exists t1. exists t2. split;[exact Hneq_t|].
+  destruct Hdouble_votes as (s1 & s1_h & s2 & s2_h & t_h & Hvote1 & Hvote2).
+  exists s1; exists s1_h; exists s2; exists s2_h; exists t_h.
+
+  rewrite in_fsetU in Hvote1;case/orP: Hvote1 => Hvote1.
+  rewrite in_fsetU in Hvote1;case/orP: Hvote1 => Hvote1.
+  split;[assumption|].
+  apply H_st_highest in Hvote1.
+
+  rewrite in_fsetU in Hvote2;case/orP: Hvote2 => Hvote2.
+  rewrite in_fsetU in Hvote2;case/orP: Hvote2 => Hvote2.
+  assumption.
+  new_vote_mem_tac Hvote2.
+  contradict Hvote1;clear. rewrite ltnn. trivial.
+  new_vote_mem_tac Hvote2.
+  contradict Hvote1;clear. rewrite ltSnn. trivial.
+
+  rewrite in_fsetU in Hvote2;case/orP: Hvote2 => Hvote2.
+  rewrite in_fsetU in Hvote2;case/orP: Hvote2 => Hvote2.
+  split;[|assumption].
+  apply H_st_highest in Hvote2.
+  new_vote_mem_tac Hvote1.
+  rewrite ltnn in Hvote2. solve[auto].
+
+  new_vote_mem_tac Hvote1.
+  new_vote_mem_tac Hvote2.
+  contradict Hneq_t. reflexivity.
+
+  new_vote_mem_tac Hvote1.
+  new_vote_mem_tac Hvote2.
+  contradict H2. solve[apply n_Sn].
+
+  rewrite in_fsetU in Hvote2;case/orP: Hvote2 => Hvote2.
+  rewrite in_fsetU in Hvote2;case/orP: Hvote2 => Hvote2.
+  split;[|assumption].
+  apply H_st_highest in Hvote2.
+  new_vote_mem_tac Hvote1.
+  contradict Hvote2;clear. rewrite ltSnn. trivial.
+
+  new_vote_mem_tac Hvote1.
+  new_vote_mem_tac Hvote2.
+  symmetry in H2. solve[case/n_Sn: H2].
+
+  new_vote_mem_tac Hvote1.
+  new_vote_mem_tac Hvote2.
+  clear -Hneq_t. congruence.
+
+  (* slashed surround case *)
+  unfold slashed_surround in Hnest |- *.
+  destruct Hnest as (s1 & t1 & s1_h & t1_h & s2 & t2 & s2_h & t2_h & Hnest).
+  exists s1;exists t1;exists s1_h;exists t1_h;exists s2;exists t2;exists s2_h;exists t2_h.
+  destruct Hnest as (Houter & Hinner & Hstarts & Hends).
+  rewrite <- and_assoc. split;[|split;assumption].
+
+  unfold vote_msg in * |- *.
+  rewrite in_fsetU in Houter;case/orP: Houter => Houter.
+  rewrite in_fsetU in Houter;case/orP: Houter => Houter.
+  split;[assumption|].
+  apply H_st_highest in Houter.
+
+  rewrite in_fsetU in Hinner;case/orP: Hinner => Hinner.
+  rewrite in_fsetU in Hinner;case/orP: Hinner => Hinner.
+  assumption.
+
+  new_vote_mem_tac Hinner.
+  clear -Hends Houter.
+  assert (t1_h < t1_h) by (apply ltn_trans with (highest_target.+1);assumption).
+  rewrite ltnn in H. contradict H. solve[trivial].
+
+  new_vote_mem_tac Hinner.
+  clear -Hends Houter.
+  assert (t1_h < t1_h).
+  apply ltn_trans with (highest_target.+1).
+  assumption. apply ltn_trans with (highest_target.+2). apply ltnSn. assumption.
+  contradict H. rewrite ltnn. solve[trivial].
+
+  rewrite in_fsetU in Hinner;case/orP: Hinner => Hinner.
+  rewrite in_fsetU in Hinner;case/orP: Hinner => Hinner.
+  split;[|assumption].
+
+  new_vote_mem_tac Houter.
+  change (is_true (badV \in good_quorum)) in x_good.
+
+  apply Hgood in x_good. destruct x_good as [Hnot_slashed Hsources_justified].
+  apply Hsources_justified in Hinner. destruct Hinner as [_ Hst2_justified].
+  clear -Hjust_max_max Hst2_justified Hstarts.
+  apply Hjust_max_max in Hst2_justified;[|apply ltnW;assumption].
+  destruct Hst2_justified.
+  contradict Hstarts. case/eqP: H0 =><-. rewrite ltnn. trivial.
+
+  new_vote_mem_tac Houter.
+  new_vote_mem_tac Hinner.
+  contradict Hstarts. clear. rewrite ltnn. trivial.
+
+  new_vote_mem_tac Houter.
+  new_vote_mem_tac Hinner.
+  contradict Hends. clear. rewrite ltSnn. trivial.
+
+  rewrite in_fsetU in Hinner;case/orP: Hinner => Hinner.
+  rewrite in_fsetU in Hinner;case/orP: Hinner => Hinner.
+  split;[|assumption].
+
+  new_vote_mem_tac Houter.
+  apply Hgood in x_good. destruct x_good as [_ x_good].
+  apply x_good in Hinner. destruct Hinner as [_ Hinner].
+  apply Hjust_le_target in Hinner.
+  clear -Hstarts Hinner.
+  rewrite <- ltnS in Hinner.
+  assert (s2_h < s2_h). apply ltn_trans with highest_target.+1;assumption.
+  contradict H. rewrite ltnn. trivial.
+
+  new_vote_mem_tac Houter.
+  new_vote_mem_tac Hinner.
+  exfalso.
+  apply Hjust_le_target in Hjust_max_just.
+  clear -Hjust_max_just Hstarts.
+  rewrite <- ltnS in Hjust_max_just.
+  assert (just_max_h < just_max_h).
+  eapply ltn_trans;eassumption.
+  contradict H. rewrite ltnn. trivial.
+
+  new_vote_mem_tac Houter.
+  new_vote_mem_tac Hinner.
+  contradict Hstarts. clear.
+  rewrite ltnn. trivial.
+Qed.
 End Liveness.
